\documentclass[a4paper]{article}

\usepackage[english]{babel}
\usepackage[utf8]{inputenc}
\usepackage{amsmath}
\usepackage{graphicx}
\usepackage[colorinlistoftodos]{todonotes}
\usepackage{geometry}
\usepackage{hyperref}
\usepackage{setspace}
\onehalfspacing

\begin{document}

\section*{Exercise 1}

For the Brock and Mirman model, find the value of A in the policy function. Show that your value is correct.

For this case find an algebraic solution for the policy function $k_{t+1} = \Phi(k_t, z_t)$. Sources for hints are Stokey et al. (1989, exercise 2.2, p. 12) and Sargent (1987, exercise 1.1, p. 47).

\subsection{Brock and Mirman's Model}

Households solve the following dynamic program:

$$ V(K_t, z_t) =  max_{K_{t+1}}ln(e^{z_t}K_t^{\alpha} - K_{t+1}) + \beta E_t\{V(K_{t+1}, z_{t+1})\}$$

The associated Euler equaation is:

$$ \frac{1}{e^{z_t}K_t^{\alpha} - K_{t+1}} =  \beta E_t\{\frac{\alpha e^{z_{t+1}}K_{t+1}^{\alpha-1}}{e^{z_{t+1}}K_{t+1}^{\alpha} - K_{t+2}}\}$$

The law of motion for z is:

$$z_{t+1} = \rho z_t + \epsilon_t \text{;   }\epsilon_t \approx i.i.d(0,\sigma^2)$$

Verify that the policy function is of the following form:

$$K_{t+1} = Ae^{z_t}K_t^{\alpha}$$

In order to determine the policy function, we need to find the value of A as a function of the model's parameters. Lets expand the euler equations:

$$ \frac{1}{e^{z_t}K_t^{\alpha} - K_{t+1}} =  \beta E_t\{\frac{\alpha e^{z_{t+1}}K_{t+1}^{\alpha-1}}{e^{z_{t+1}}K_{t+1}^{\alpha}*(1-A)}\}$$

$$ \iff \frac{1}{e^{z_t}K_t^{\alpha} - K_{t+1}} =  \beta E_t\{\frac{\alpha K_{t+1}^{\alpha-1}}{K_{t+1}^{\alpha}*(1-A)}\}$$

$$ \iff \frac{1}{e^{z_t}K_t^{\alpha} - K_{t+1}} =  \beta E_t\{\frac{\alpha}{K_{t+1}(1-A)}\}$$

$$ \iff \frac{1}{e^{z_t}K_t^{\alpha} - K_{t+1}} =  \beta \frac{\alpha}{K_{t+1}(1-A)}$$

$$ \iff 1 =  \beta*\alpha \frac{e^{z_t}K_t^{\alpha} - K_{t+1}}{K_{t+1}(1-A)}$$

$$ \iff A=  \beta*\alpha $$

\section*{Exercise 2}

$$ u = a \log{\left(1 - l_{t} \right)} + \log{\left(c_{t} \right)} $$
$$ F =  K_{t}^{\alpha} L_{t}^{1 - \alpha} e^{z} $$
$$ du/dc =  \frac{1}{c_{t}} $$
$$ du/dl =  - \frac{a}{1 - l_{t}} $$
$$ E1 \text{  }
 0 =  T_{t} - c_{t} + k_{t} - k_{t+1} + \left(1 - \tau\right) \left(k_{t} \left(- \delta + r_{t}\right) + l_{t} w_{t}\right) $$
$$ E2 \text{  }
 0 =  \frac{\beta \left(\left(1 - \tau\right) \left(- \delta + r_{t+1}\right) + 1\right)}{c_{t+1}} - \frac{1}{c_{t}} $$
$$ E3 \text{  }
 0 =  - \frac{a}{1 - l_{t}} + \frac{w_{t} \left(1 - \tau\right)}{c_{t}} $$
$$ E4 \text{  }
 0 =  - \frac{\alpha k_{t}^{\alpha} l_{t}^{1 - \alpha} e^{z}}{k_{t}} + r_{t} $$
$$ E5 \text{  }
 0 =  - \frac{k_{t}^{\alpha} l_{t}^{1 - \alpha} \left(1 - \alpha\right) e^{z}}{l_{t}} + w_{t} $$
$$ E6 \text{  }
 0 =  T_{t} - \tau \left(k_{t} \left(- \delta + r_{t}\right) + l_{t} w_{t}\right) $$


\section*{Exercise 3}

$$ u =  a \log{\left(1 - l_{t} \right)} + \frac{c_{t}^{1 - \gamma} - 1}{1 - \gamma} $$
$$ F =  k_{t}^{\alpha} l_{t}^{1 - \alpha} e^{z} $$
$$ du/dc =  \frac{c_{t}^{1 - \gamma}}{c_{t}} $$
$$ du/dl =  - \frac{a}{1 - l_{t}} $$
$$ E1 \text{  }
 0 =  T_{t} - c_{t} + k_{t} - k_{t+1} + \left(1 - \tau\right) \left(k_{t} \left(- \delta + r_{t}\right) + l_{t} w_{t}\right) $$
$$ E2 \text{  }
 0 =  \frac{\beta c_{t+1}^{1 - \gamma} \left(\left(1 - \tau\right) \left(- \delta + r_{t+1}\right) + 1\right)}{c_{t+1}} - \frac{c_{t}^{1 - \gamma}}{c_{t}} $$
$$ E3 \text{  }
 0 =  - \frac{a}{1 - l_{t}} + \frac{c_{t}^{1 - \gamma} w_{t} \left(1 - \tau\right)}{c_{t}} $$
$$ E4 \text{  }
 0 =  - \frac{\alpha k_{t}^{\alpha} l_{t}^{1 - \alpha} e^{z}}{k_{t}} + r_{t} $$
$$ E5 \text{  }
 0 =  - \frac{k_{t}^{\alpha} l_{t}^{1 - \alpha} \left(1 - \alpha\right) e^{z}}{l_{t}} + w_{t} $$
$$ E6 \text{  }
 0 =  T_{t} - \tau \left(k_{t} \left(- \delta + r_{t}\right) + l_{t} w_{t}\right) $$

\section*{Exercise 4}

$$ u =  \frac{a \left(\left(1 - l_{t}\right)^{1 - \xi} - 1\right)}{1 - \xi} + \frac{c_{t}^{1 - \gamma} - 1}{1 - \gamma} $$
$$ F =  \left(\alpha k_{t}^{\eta} + l_{t}^{\eta} \left(1 - \alpha\right)\right)^{\frac{1}{\eta}} e^{z} $$
$$ du/dc =  \frac{c_{t}^{1 - \gamma}}{c_{t}} $$
$$ du/dl =  \frac{a \left(1 - l_{t}\right)^{1 - \xi} \left(\xi - 1\right)}{\left(1 - \xi\right) \left(1 - l_{t}\right)} $$
$$ E1 \text{  }
 0 =  T_{t} - c_{t} + k_{t} - k_{t+1} + \left(1 - \tau\right) \left(k_{t} \left(- \delta + r_{t}\right) + l_{t} w_{t}\right) $$
$$ E2 \text{  }
 0 =  \frac{\beta c_{t+1}^{1 - \gamma} \left(\left(1 - \tau\right) \left(- \delta + r_{t+1}\right) + 1\right)}{c_{t+1}} - \frac{c_{t}^{1 - \gamma}}{c_{t}} $$
$$ E3 \text{  }
 0 =  \frac{a \left(1 - l_{t}\right)^{1 - \xi} \left(\xi - 1\right)}{\left(1 - \xi\right) \left(1 - l_{t}\right)} + \frac{c_{t}^{1 - \gamma} w_{t} \left(1 - \tau\right)}{c_{t}} $$
$$ E4 \text{  }
 0 =  - \frac{\alpha k_{t}^{\eta} \left(\alpha k_{t}^{\eta} + l_{t}^{\eta} \left(1 - \alpha\right)\right)^{\frac{1}{\eta}} e^{z}}{k_{t} \left(\alpha k_{t}^{\eta} + l_{t}^{\eta} \left(1 - \alpha\right)\right)} + r_{t} $$
$$ E5 \text{  }
 0 =  w_{t} - \frac{l_{t}^{\eta} \left(1 - \alpha\right) \left(\alpha k_{t}^{\eta} + l_{t}^{\eta} \left(1 - \alpha\right)\right)^{\frac{1}{\eta}} e^{z}}{l_{t} \left(\alpha k_{t}^{\eta} + l_{t}^{\eta} \left(1 - \alpha\right)\right)} $$
$$ E6 \text{  }
 0 =  T_{t} - \tau \left(k_{t} \left(- \delta + r_{t}\right) + l_{t} w_{t}\right) $$

\section*{Exercise 5}
$$ u =  \frac{c_{t}^{1 - \gamma} - 1}{1 - \gamma} $$
$$ F =  k_{t}^{\alpha} \left(l_{t} e^{z}\right)^{1 - \alpha} $$
$$ du/dc  =  \frac{c_{t}^{1 - \gamma}}{c_{t}} $$
$$ du/dl  =  0 $$

Equilibrium equations:
$$ E1 \text{  }
 0 =  T_{t} - c_{t} + k_{t} - k_{t+1} + \left(1 - \tau\right) \left(k_{t} \left(- \delta + r_{t}\right) + l_{t} w_{t}\right) $$
$$ E2 \text{  }
 0 =  \frac{\beta c_{t+1}^{1 - \gamma} \left(\left(1 - \tau\right) \left(- \delta + r_{t+1}\right) + 1\right)}{c_{t+1}} - \frac{c_{t}^{1 - \gamma}}{c_{t}} $$
$$ E3 \text{  }
 0 =  \frac{c_{t}^{1 - \gamma} w_{t} \left(1 - \tau\right)}{c_{t}} $$
$$ E4 \text{  }
 0 =  - \frac{\alpha k_{t}^{\alpha} \left(l_{t} e^{z}\right)^{1 - \alpha}}{k_{t}} + r_{t} $$
$$ E5 \text{  }
 0 =  - \frac{k_{t}^{\alpha} \left(l_{t} e^{z}\right)^{1 - \alpha} \left(1 - \alpha\right)}{l_{t}} + w_{t} $$
$$ E6 \text{  }
 0 =  T_{t} - \tau \left(k_{t} \left(- \delta + r_{t}\right) + l_{t} w_{t}\right) $$

Steady state equations:

$$ E1 \text{  }
 0 =  T - c + \left(1 - \tau\right) \left(k \left(- \delta + r\right) + l w\right) $$
$$ E2 \text{  }
 0 =  \frac{c^{1 - \gamma} \left(- \beta \left(\left(1 - \tau\right) \left(- \delta + r\right) + 1\right) + 1\right)}{c} $$
$$ E3 \text{  }
 0 =  \frac{c^{1 - \gamma} w \left(1 - \tau\right)}{c} $$
$$ E4 \text{  }
 0 =  r - \frac{K^{\alpha} \alpha \left(L e^{z}\right)^{1 - \alpha}}{K} $$
$$ E5 \text{  }
 0 =  - \frac{K^{\alpha} \left(L e^{z}\right)^{1 - \alpha} \left(1 - \alpha\right)}{L} + w $$
$$ E6 \text{  }
 0 =  T - \tau \left(k \left(- \delta + r\right) + l w\right) $$
\section*{Exercise 6}
Steady state equations:
$$ u \text{  }
 0 =  \frac{a \left(\left(1 - l\right)^{1 - \xi} - 1\right)}{1 - \xi} + \frac{c^{1 - \gamma} - 1}{1 - \gamma} $$
$$ F \text{  }
 0 =  K^{\alpha} \left(L e^{z}\right)^{1 - \alpha} $$
$$ du/dc \text{  }
 0 =  \frac{c^{1 - \gamma}}{c} $$
$$ du/dl \text{  }
 0 =  \frac{a \left(1 - l\right)^{1 - \xi} \left(\xi - 1\right)}{\left(1 - \xi\right) \left(1 - l\right)} $$
$$ E1 \text{  }
 0 =  T - c + \left(1 - \tau\right) \left(k \left(- \delta + r\right) + l w\right) $$
$$ E2 \text{  }
 0 =  \frac{c^{1 - \gamma} \left(- \beta \left(\left(1 - \tau\right) \left(- \delta + r\right) + 1\right) + 1\right)}{c} $$
$$ E3 \text{  }
 0 =  \frac{a \left(1 - l\right)^{1 - \xi} \left(\xi - 1\right)}{\left(1 - \xi\right) \left(1 - l\right)} + \frac{c^{1 - \gamma} w \left(1 - \tau\right)}{c} $$
$$ E4 \text{  }
 0 =  r - \frac{K^{\alpha} \alpha \left(L e^{z}\right)^{1 - \alpha}}{K} $$
$$ E5 \text{  }
 0 =  - \frac{K^{\alpha} \left(L e^{z}\right)^{1 - \alpha} \left(1 - \alpha\right)}{L} + w $$
$$ E6 \text{  }
 0 =  T - \tau \left(k \left(- \delta + r\right) + l w\right) $$



\section*{Exercise 7}

For the steady state of the baseline tax model in section 3.7.3 use numerican differentiation to solve for the full set of comparative statics and sign them where possible.
∂y  ̄ ̄  ̄ ̄
Find ∂x for y ∈ {k,l,y ̄,w ̄,r ̄,T,i,c ̄} and x ∈ {α,β,γ,δ,ξ,τ,a,z ̄}.
Using the same parameter values as in excercise 6, solve for the numerical values of the comparative statics.

\end{document}
